secure_api/merkle_tree/MerkleTree.New.Low.fst
@@ -389,7 +389,7 @@ private let rec insert_ lv i j hs acc =
 	       hs acc)
 
 // Caution: current impl. manipulates the content in `v`.
-val insert:
+val mt_insert:
   mt:mt_p -> v:hash ->
   HST.ST unit
 	 (requires (fun h0 ->
@@ -400,7 +400,7 @@ val insert:
 	 (ensures (fun h0 _ h1 ->
 	   modifies (mt_loc mt) h0 h1 /\
 	   mt_safe h1 mt))
-let rec insert mt v =
+let mt_insert mt v =
   let mtv = B.index mt 0ul in
   insert_ 0ul (Ghost.hide (MT?.i mtv)) (MT?.j mtv) (MT?.hs mtv) v;
   B.upd mt 0ul 
@@ -412,7 +412,6 @@ let rec insert mt v =
 
 /// Getting the Merkle root and path
 
-// b:uint8_p{B.len b = U32.mul 32ul hash_size}
 type path = B.pointer (V.vector hash)
 
 val path_safe: HS.mem -> path -> GTot Type0
@@ -424,7 +423,7 @@ let path_safe h p =
 // Construct the rightmost hashes for a given (incomplete) Merkle tree.
 // This function calculates the Merkle root as well, which is the final
 // accumulator value.
-val construct_rhs:
+private val construct_rhs:
   lv:uint32_t{lv < 32ul} ->
   hs:hash_vv{V.size_of hs = 32ul} ->
   rhs:hash_vec{V.size_of rhs = 32ul} ->
@@ -442,7 +441,7 @@ val construct_rhs:
 	 (ensures (fun h0 _ h1 ->
 	   modifies (RV.loc_rvector rhs) h0 h1 /\
 	   RV.rv_inv h1 rhs))
-let rec construct_rhs lv hs rhs i j acc actd =
+private let rec construct_rhs lv hs rhs i j acc actd =
   admit ();
   let ofs = offset_of i in
   let copy = Cpy?.copy hcpy in
@@ -458,11 +457,27 @@ let rec construct_rhs lv hs rhs i j acc actd =
 	 else (copy (V.index (V.index hs lv) (j - 1ul - ofs)) acc);
 	 construct_rhs (lv + 1ul) hs rhs (i / 2ul) (j / 2ul) acc true))
 
+val mt_get_root:
+  mt:mt_p -> 
+  root:hash ->
+  HST.ST unit
+	 (requires (fun h0 -> true))
+	 (ensures (fun h0 _ h1 -> true))
+let mt_get_root mt root =
+  admit ();
+  let mtv = B.index mt 0ul in
+  let i = MT?.i mtv in
+  let j = MT?.j mtv in
+  let hs = MT?.hs mtv in
+  let rhs = MT?.rhs mtv in
+  construct_rhs 0ul hs rhs i j root false;
+  B.upd mt 0ul (MT i j hs true rhs)
+
 // Construct a Merkle path for a given index `k`, hashes `hs`, 
 // and rightmost hashes `rhs`.
 // Caution: current impl. copies "pointers" in the Merkle tree 
 //          to the output path.
-val mt_get_path_:
+private val mt_get_path_:
   lv:uint32_t{lv < 32ul} ->
   hs:hash_vv{V.size_of hs = 32ul} ->
   rhs:hash_vec{V.size_of rhs = 32ul} ->
@@ -475,32 +490,30 @@ val mt_get_path_:
 	   HH.disjoint (V.frameOf hs) (V.frameOf rhs) /\
 	   mt_safe_elts h0 lv hs i j))
 	 (ensures (fun h0 _ h1 -> true))
-let rec mt_get_path_ lv hs rhs i j k p =
+private let rec mt_get_path_ lv hs rhs i j k p =
   admit ();
   let ofs = offset_of i in
   if j = 0ul then ()
   else
-    (if k % 2ul = 1ul
-    then B.upd p 0ul (V.insert (B.index p 0ul)
-				  (V.index (V.index hs lv) (k - 1ul - ofs)))
+    (let pv = B.index p 0ul in
+    if k % 2ul = 1ul
+    then B.upd p 0ul (V.insert pv (V.index (V.index hs lv) (k - 1ul - ofs)))
     else
       (if k = j then ()
       else if k + 1ul = j
-      then B.upd p 0ul (V.insert (B.index p 0ul) (V.index rhs lv))
-      else B.upd p 0ul (V.insert (B.index p 0ul)
-  	 			    (V.index (V.index hs lv) (k + 1ul - ofs))));
+      then B.upd p 0ul (V.insert pv (V.index rhs lv))
+      else B.upd p 0ul (V.insert pv (V.index (V.index hs lv) (k + 1ul - ofs))));
     mt_get_path_ (lv + 1ul) hs rhs (i / 2ul) (j / 2ul) (k / 2ul) p)
 
 val mt_get_path:
   mt:mt_p -> 
   idx:uint32_t -> // {MT?.i mt <= idx && idx < MT?.j mt}
-  ih:hash ->
   p:path ->
   root:hash ->
   HST.ST uint32_t
 	 (requires (fun h0 -> true))
 	 (ensures (fun h0 _ h1 -> true))
-let mt_get_path mt idx ih p root =
+let mt_get_path mt idx p root =
   admit ();
   let copy = Cpy?.copy hcpy in
   let mtv = B.index mt 0ul in
@@ -514,20 +527,21 @@ let mt_get_path mt idx ih p root =
     construct_rhs 0ul hs rhs i j root false;
     B.upd mt 0ul (MT i j hs true rhs))
   else ();
+  let ih = V.index (V.index hs 0ul) (idx - ofs) in
+  B.upd p 0ul (RV.insert_copy hcpy (B.index p 0ul) ih);
   mt_get_path_ 0ul hs rhs i (j - 1) idx p;
-  copy (V.index (V.index hs 0ul) (idx - ofs)) ih;
   j
 
 /// Flushing
 
-val mt_flush_to_:
+private val mt_flush_to_:
   lv:uint32_t{lv < 32ul} ->
   hs:hash_vv{V.size_of hs = 32ul} ->
   i:uint32_t ->
   HST.ST unit
 	 (requires (fun h0 -> true))
 	 (ensures (fun h0 _ h1 -> true))
-let rec mt_flush_to_ lv hs i =
+private let rec mt_flush_to_ lv hs i =
   admit ();
   if i = 0ul then ()
   else (let ofs = offset_of i in
@@ -562,7 +576,7 @@ let mt_flush mt =
 
 /// Client-side verification
 
-val mt_verify_:
+private val mt_verify_:
   k:uint32_t ->
   j:uint32_t{j = 0ul || k <= j} ->
   p:path ->
@@ -573,7 +587,7 @@ val mt_verify_:
 	   path_safe h0 p /\
 	   ppos < V.size_of (B.get h0 p 0)))
 	 (ensures (fun h0 _ h1 -> true))
-let rec mt_verify_ k j p ppos acc =
+private let rec mt_verify_ k j p ppos acc =
   admit ();
   if j <= 1ul then ()
   else (let phash = V.index (B.index p 0ul) ppos in
@@ -585,7 +599,7 @@ let rec mt_verify_ k j p ppos acc =
        else (hash_2 phash acc acc;
 	    mt_verify_ (k / 2ul) ((j + 1ul) / 2ul) p (ppos + 1ul) acc))
 
-val buf_eq:
+private val buf_eq:
   #a:eqtype -> b1:B.buffer a -> b2:B.buffer a ->
   len:uint32_t ->
   HST.ST bool
@@ -593,7 +607,7 @@ val buf_eq:
 	   B.live h0 b1 /\ B.live h0 b2 /\
 	   len <= B.len b1 /\ len <= B.len b2))
 	 (ensures (fun h0 _ h1 -> true))
-let rec buf_eq #a b1 b2 len =
+private let rec buf_eq #a b1 b2 len =
   if len = 0ul then true
   else (let a1 = B.index b1 (len - 1ul) in
        let a2 = B.index b2 (len - 1ul) in
@@ -603,14 +617,16 @@ let rec buf_eq #a b1 b2 len =
 val mt_verify:
   k:uint32_t ->
   j:uint32_t{k < j} ->
-  ih:hash ->
   p:path ->
   root:hash ->
   HST.ST bool
 	 (requires (fun h0 -> true))
 	 (ensures (fun h0 _ h1 -> true))
-let mt_verify k j ih p root =
+let mt_verify k j p root =
   admit ();
-  mt_verify_ k j p 0ul ih;
+  let ih = hash_r_init HH.root in
+  let copy = Cpy?.copy hcpy in
+  copy (V.index (B.index p 0ul) 0ul) ih;
+  mt_verify_ k j p 1ul ih;
   buf_eq ih root hash_size
 
